# More hyperbolic functions

$\text{arsinh}x = \ln(x + \sqrt{x^2 + 1})$

$\text{arsinh}7 = 2.644$

$\cosh^2(x) - \cosh x -2 = 0$  
$t = \cosh x$  
$t^2 - t - 2 = 0$  
$t \in \{2, -1\}$  
$\text{arcosh} t \in{1.317, -1.317}$ (arcosh of -1 is invalid, but 2 has 2
solutions)

---

$\tanh x = \frac{\sinh x}{\cosh x}$  
$\tanh \text{artanh} (x) = (x)$

If $\text{artanh} = \frac{1}{2}\ln (\frac{1+x}{1-x})$ the above will be true for
it...  
$\tanh \text{artanh} x= \frac{\frac{e^{\frac{1}{2}\ln(\frac{1 + x}{1 - x})} -
e^{-{\frac{1}{2}\ln(\frac{1 + x}{1 - x})}}}{2}}{\frac{e^{\frac{1}{2}\ln(
\frac{1 + x}{1 - x})} + e^{-\frac{1}{2}\ln(\frac{1 + x}{1 - x})}}{2}}$  
$= \frac{e^{\frac{1}{2}\ln(\frac{1 + x}{1 - x})} -
e^{-{\frac{1}{2}\ln(\frac{1 + x}{1 - x})}}}{e^{\frac{1}{2}\ln(
\frac{1 + x}{1 - x})} + e^{-\frac{1}{2}\ln(\frac{1 + x}{1 - x})}}$  
$=\frac{1 - e^{-1}}{1 + e^{-1}}$

---

$\tanh2x = \frac{\sinh2x}{\cosh2x}$  
$\tanh2x = \frac{2\sinh x\cosh x}{\cosh^2 x + \sinh^2 x}$  
$\tanh2x = \frac{2\sinh x\cosh x(\frac{1}{\cosh^2 x})}{1 + \tanh^2x}$  
$\tanh2x = \frac{2\sinh x(\frac{1}{\cosh x})}{1 + \tanh^2x}$  
$\tanh2x = \frac{2\tanh x}{1 + \tanh^2x}$

---

$5\sinh x - 4\cosh x = 0$  
$5(\frac{e^x - e^{-x}}{2}) - 4(\frac{e^x + e^{-x}}{2}) = 0$  
$\frac{5}{2}(e^x - e^{-x}) - 2(e^x + e^{-x}) = 0$  
$\frac{5}{2}e^x - \frac{5}{2}e^{-x} - 2e^x - 2e^{-x}=0$  
$\frac{1}{2}e^x -\frac{9}{2}e^{-x}=0$  
$\frac{1}{2}\ln x = \frac{9}{2}\ln(-x)$  
$\ln x = 9\ln(-x)$

---

$\sinh x + \sinh y = \frac{21}{8}$  
$\cosh x + \cosh y = \frac{27}{8}$

$\frac{e^x - e^{-x}}{2}+\frac{e^y - e^{-y}}{2} = \frac{21}{8}$  
$\frac{e^x + e^{-x}}{2}+\frac{e^y + e^{-y}}{2} = \frac{27}{8}$

$e^x - e^{-x}+e^y - e^{-y} = \frac{21}{4}$  
$e^x + e^{-x}+e^y + e^{-y} = \frac{27}{4}$

$e^x+e^x*e^{-1}+e^y+e^y*e^{-1}=\frac{27}{4}$  
$e^x-e^x*e^{-1}+e^y-e^y*e^{-1}=\frac{21}{4}$

---


